stdlib/lampe/Stdlib/Extra.lean
@@ -1,0 +1,12 @@
+import Lampe
+
+/-!
+Theorems for Lean's builtin types that are needed to prove the standard library functionality. 
+-/
+
+namespace Lampe.Stdlib
+
+set_option Lampe.pp.Expr false
+set_option Lampe.pp.STHoare false
+
+theorem Ordering.then_of_ne_eq (hp: o₁ ≠ .eq) : Ordering.then o₁ o₂ = o₁ := by cases o₁ <;> simp_all
